Phi_OO.thy
@@ -243,13 +243,13 @@ paragraph \<open>Allocation\<close>
 definition (in \<phi>OO_sem) op_obj_allocate :: \<open>'TY class \<Rightarrow> ('VAL,'RES_N,'RES) proc\<close>
   where \<open>op_obj_allocate cls =
       R_objs.\<phi>R_allocate_res_entry (\<lambda>ref. ref \<noteq> Nil \<and> object_ref.class ref = cls)
-            (initial_value_of_class cls) (\<lambda>ref. Success (sem_value (V_ref.mk ref)))\<close>
+            (initial_value_of_class cls) (\<lambda>ref. Return (sem_value (V_ref.mk ref)))\<close>
 
 lemma (in \<phi>OO) op_obj_allocate:
   \<open>\<^bold>p\<^bold>r\<^bold>o\<^bold>c op_obj_allocate cls
       \<lbrace> Void \<longmapsto> \<lambda>ret. \<exists>*ref. to_share o initial_value_of_class cls \<Ztypecolon> \<phi>RawObject ref\<heavy_comma> ref \<Ztypecolon> Val ret (Ref cls) \<rbrace>\<close>
   unfolding \<phi>Procedure_\<phi>Res_Spec op_obj_allocate_def
-  apply (clarsimp simp add: \<phi>expns FIC_OO_share.interp_split')
+  apply (clarsimp simp add: \<phi>expns FIC_OO_share.interp_split' del: subsetI)
   apply (rule R_objs.\<phi>R_allocate_res_entry)
   apply (clarsimp simp add: Valid_Objs_def)
   using obj_map_freshness apply blast
@@ -257,7 +257,7 @@ lemma (in \<phi>OO) op_obj_allocate:
   prefer 2 apply assumption
   apply (simp add: \<phi>expns)
   subgoal for r res k res'
-    by (cases k; simp add: R_objs.share_fiction_expn_full') .
+    by (cases k; simp add: R_objs.share_fiction_expn_full' Return_def det_lift_def) .
 
 
 
@@ -267,7 +267,7 @@ definition (in \<phi>OO_sem) op_obj_load_field :: \<open>field_name \<Rightarrow
   where \<open>op_obj_load_field field TY v =
     \<phi>M_getV_ref v (\<lambda>ref.
     R_objs.\<phi>R_get_res_entry ref field (\<lambda>v.
-    \<phi>M_assert (v \<in> Well_Type TY) \<ggreater> Success (sem_value v)))\<close>
+    \<phi>M_assert (v \<in> Well_Type TY) \<ggreater> Return (sem_value v)))\<close>
 
 lemma (in \<phi>OO) \<phi>M_get_res_entry_R_objs[\<phi>reason!]:
   \<open>\<^bold>p\<^bold>r\<^bold>o\<^bold>c F v
@@ -275,7 +275,7 @@ lemma (in \<phi>OO) \<phi>M_get_res_entry_R_objs[\<phi>reason!]:
 \<Longrightarrow> \<^bold>p\<^bold>r\<^bold>o\<^bold>c R_objs.\<phi>R_get_res_entry ref field F
       \<lbrace> v \<Ztypecolon> \<phi>InObj ref (\<phi>MapAt field (n \<Znrres>\<phi> Identity)) \<longmapsto> Y \<^bold>t\<^bold>h\<^bold>r\<^bold>o\<^bold>w\<^bold>s E \<rbrace>\<close>
   unfolding \<phi>Procedure_\<phi>Res_Spec
-  apply (clarsimp simp add: \<phi>expns zero_set_def)
+  apply (clarsimp simp add: \<phi>expns zero_set_def del: subsetI)
   apply (rule R_objs.\<phi>R_get_res_entry[where v=v])
    apply (simp add: FIC_OO_share.interp_split')
   by blast
@@ -308,7 +308,7 @@ lemma (in \<phi>OO) "\<phi>R_set_res_objs"[\<phi>reason!]:
   \<longmapsto> \<lambda>\<r>\<e>\<t>. u \<Ztypecolon> \<phi>InObj ref (\<phi>MapAt field (1 \<Znrres>\<phi> Identity)) \<rbrace>\<close>
   unfolding \<phi>Procedure_\<phi>Res_Spec
   apply (clarsimp simp add: \<phi>expns zero_set_def FIC_OO_share.interp_split'
-          R_objs.share_fiction_expn_full)
+          R_objs.share_fiction_expn_full del: subsetI)
   apply (rule R_objs.\<phi>R_set_res[where P="\<lambda>m. field \<in> dom (m ref)"])
   apply (cases ref; clarsimp simp add: Valid_Objs_def map_fun_at_def dom1_def)
   apply (smt (verit, del_insts) Collect_cong dom_1 dom_eq_empty_conv insert_dom option.distinct(1))
@@ -347,7 +347,7 @@ lemma (in \<phi>OO) op_obj_dispose:
   apply (rule \<phi>SEQ[where B=\<open>\<lambda>_. to_share \<circ> fields \<Ztypecolon> \<phi>RawObject ref\<close>])
   unfolding \<phi>Procedure_\<phi>Res_Spec
   apply (clarsimp simp add: \<phi>expns zero_set_def FIC_OO_share.interp_split'
-          R_objs.share_fiction_expn_full')
+          R_objs.share_fiction_expn_full' del: subsetI)
    apply (rule R_objs.\<phi>R_get_res, simp, simp add: dom1_def)
   subgoal premises prems for r res proof -
     have t1: \<open>object_ref.class ref = cls\<close>
@@ -356,10 +356,10 @@ lemma (in \<phi>OO) op_obj_dispose:
       unfolding one_fun_def one_option_def
       using R_objs.raw_unit_assertion_implies'[unfolded map_le_def, OF \<open>res \<in> _\<close>]
       by (metis domIff prems(2))
-    show ?thesis by (simp add: t1 t2 prems)
+    show ?thesis by (simp add: t1 t2 prems Return_def det_lift_def)
   qed
   apply (clarsimp simp add: \<phi>expns zero_set_def FIC_OO_share.interp_split'
-          R_objs.share_fiction_expn_full')
+          R_objs.share_fiction_expn_full' del: subsetI)
   apply (rule R_objs.\<phi>R_dispose_res[where P=\<open>\<lambda>_. True\<close> and any=fields])
      apply (clarsimp simp add: Valid_Objs_def one_fun_def)
   apply (cases ref; simp)
